WIP

pulse/examples/steel/LList.Invariant.fst
@@ -40,7 +40,7 @@ let mk_cell (n: t 'a) (d:'a) = {
 let hd l = Cons?.hd l
 let tl l = Cons?.tl l
 
-let null_llist (#a:Type)  = admit()
+let null_llist (#a:Type)  = null
 let ptr_eq (#a:Type) (x y:t a) = admit()
 
 
@@ -61,6 +61,40 @@ let rec llist' (#a:Type) (ptr:t a)
       llist' (next hd) tl
 let llist = llist'
 
+let rec llist_fragment' (#a:Type) (ptr:t a)
+                         (l:list (cell a))
+    : Tot slprop (decreases l)
+    =
+    match l with
+    | [] -> emp
+
+    | hd :: tl ->
+      pure (ptr =!= null_llist) `star`
+      pts_to ptr full_perm hd `star`
+      llist_fragment' (next hd) tl
+
+let llist2  (#a:Type) (ptr:t a)
+                      (l:list (cell a))
+: Tot slprop
+= llist_fragment' ptr l `star`
+  begin if Nil? l
+  then pure (ptr == null_llist)
+  else pure (next (L.last l) == null)
+  end
+
+let rec llist2_elim (#a:Type) (ptr:t a)
+                      (l:list (cell a)) (m: mem) : Lemma
+                      (requires True)
+    (ensures (interp (llist2 ptr l) m ==> interp (llist ptr l) m))
+    (decreases l)
+= match l with
+  | [] ->
+    norm_spec [delta; zeta] (llist ptr []);
+    norm_spec [delta; zeta] (llist2 ptr [])
+  | a :: q -> 
+    norm_spec [delta; zeta] (llist ptr (a :: q));
+    norm_spec [delta; zeta] (llist2 ptr (a :: q));
+    llist2_elim (next a) q m
 
 (* Helper lemmas/rewritings *)
 
